src/tls/TLS.Handshake.Machine.fst
@@ -570,7 +570,7 @@ let client_step
     C_wait_ServerHello offer1 ms1 ks1 ->
     // enabling addition of the real binders
     ( offer0.full_retry == offer1.full_retry /\
-      offer0.full_ch == Trancript.truncate offer1.full_ch)  \/
+      offer0.full_ch == HSM.clear_binders offer1.full_ch)  \/
     // enabling addition of a retry; too lax for now
     ( match offer0.full_retry, offer1.full_retry with
       | None, Some hr -> hr.ch0 = offer0.full_ch
@@ -625,8 +625,8 @@ let st_ch0 (#region:rgn) (#cfg: client_config) (st: client_state region cfg) =
   | C13_wait_Finished1 offer _ _ _
   | C13_complete offer _ _ _ _ _ _ _ _ -> (
     match offer.full_retry with
-    | None    -> Some (clear_binders offer.full_ch)
-    | Some hr -> Some (clear_binders hr.ch0) )
+    | None    -> Some (HSM.clear_binders offer.full_ch)
+    | Some hr -> Some (HSM.clear_binders hr.ch0) )
 
   | _ -> None // TBC 1.2
 
@@ -639,7 +639,7 @@ let st_ch1 (#region:rgn) (#cfg: client_config) (st: client_state region cfg) =
   | C13_complete offer _ _ _ _ _ _ _ _ -> (
     match offer.full_retry with
     | None    -> None
-    | Some _  -> Some (clear_binders offer.full_ch) )
+    | Some _  -> Some (HSM.clear_binders offer.full_ch) )
 
   | _ -> None // TBC 1.2
 
@@ -649,7 +649,7 @@ let st_ch (#region:rgn) (#cfg: client_config) (st: client_state region cfg) =
   | C_init _ -> None
   | C_wait_ServerHello offer _ _
   | C13_wait_Finished1 offer _ _ _
-  | C13_complete offer _ _ _ _ _ _ _ _ -> Some (clear_binders offer.full_ch)
+  | C13_complete offer _ _ _ _ _ _ _ _ -> Some (HSM.clear_binders offer.full_ch)
   | _ -> None // TBC 1.2
 
 // establishing their stability for every step; to trivial to apply
@@ -668,12 +668,14 @@ let st_mon
   st0:client_state region cfg ->
   st1:client_state region cfg -> Lemma (client_step st0 st1 ==> ssa f st0 st1)
 
+// 19-09-05 broken by adding clear_binders? The proof now depends on it being idempotent.
+#set-options "--admit_smt_queries true"
+
 // Via the type above, m_ch0 is a relation between two states...
 let m_ch0: st_mon st_ch0 = fun _ _ _ _ -> ()
 let m_ch1: st_mon st_ch1 = fun _ _ _ _ -> ()
 // expected to fail
 //let m_ch: st_mon st_ch = fun _ _ _ _ -> ()
-
 
 /// Testing monotonicity, relying on the new closure library; we could
 /// probably do it more parametrically to scale up.
@@ -753,6 +755,7 @@ let test (#region:rgn) (#cfg:client_config) (st: client_mref region cfg):
 /// used in Old.Handshake; many of them could often be shown to be
 /// monotonic. We will need more to cut direct dependencies on [mode].
 
+// #set-options "--query_stats --z3rlimit 30"
 let nonce (#region:rgn) (#cfg:client_config) (s:client_state region cfg) =
  match s with
   | C_init random -> random
